more efficient freshness using var_shift

Metatheory_Var.v
@@ -4,7 +4,7 @@
 ***************************************************************************)
 
 Set Implicit Arguments.
-Require Import List Max Omega OrderedType OrderedTypeEx.
+Require Import List ZArith Omega OrderedType OrderedTypeEx.
 Require Import Lib_Tactic Lib_ListFacts Lib_FinSet Lib_FinSetImpl.
 Require Export Lib_ListFactsMore.
 
@@ -34,14 +34,27 @@ Definition vars := VarSet.S.t.
 
 (** Finally, we have a means of generating fresh variables. *)
 
-Parameter var_generate : vars -> var.
+Parameter vars_rep : vars -> var.
+Parameter var_shift : var -> positive -> var.
+Definition var_generate L := var_shift (vars_rep L) 1.
 Parameter var_generate_spec : forall E, (var_generate E) \notin E.
 Parameter var_fresh : forall (L : vars), { x : var | x \notin L }.
+Parameter var_is_fresh : forall L, proj1_sig (var_fresh L) = var_generate L.
+
+Parameter var_max : var -> var -> var.
+Parameter var_singleton : forall v, vars_rep {{v}} = v.
+Parameter var_union : forall L1 L2,
+  vars_rep (L1 \u L2) = var_max (vars_rep L1) (vars_rep L2).
+Parameter var_add : forall L,
+  vars_rep (L \u {{var_generate L}}) = var_generate L.
 
 (** Variables can be enumerated *)
 
 Parameter var_of_Z : Z -> var.
 Parameter Z_of_var : var -> Z.
+Parameter Z_of_var_inj : forall v, var_of_Z (Z_of_var v) = v.
+Parameter var_max_hom : forall v w,
+  Z_of_var (var_max v w) = Zmax (Z_of_var v) (Z_of_var w).
 
 End VARIABLES.
 
@@ -51,16 +64,26 @@ End VARIABLES.
 
 Module Variables : VARIABLES.
 
-Open Scope Z_scope.
+Open Scope positive_scope.
 
-Definition var := Z.
+Definition var := positive.
 
-Definition var_default : var := 0.
+Definition var_default : var := 1.
 
-Definition var_of_Z x : var := x.
-Definition Z_of_var x : Z := x.
+Definition var_of_Z x : var :=
+  match x with
+  | Zpos n => n
+  | Z0 => var_default
+  | Zneg n => n
+  end.
+Definition Z_of_var (x : var) : Z := Zpos x.
 
-Module Var_as_OT := Z_as_OT.
+Lemma Z_of_var_inj : forall v, var_of_Z (Z_of_var v) = v.
+Proof.
+  intros. reflexivity.
+Qed.
+
+Module Var_as_OT := Positive_as_OT.
 
 Module Import VarSet : FinSet with Module E := Var_as_OT :=
   Lib_FinSetImpl.Make Var_as_OT.
@@ -68,51 +91,257 @@ Open Local Scope set_scope.
 
 Definition vars := VarSet.S.t.
 
-Lemma max_lt_l :
-  forall (x y z : Z), x <= y -> x <= Zmax y z.
+Definition var_max p q :=
+  match (p ?= q) Eq with
+  | Gt => p
+  | Eq => p
+  | Lt => q
+  end.
+
+Lemma var_max_hom : forall v w,
+  Z_of_var (var_max v w) = Zmax (Z_of_var v) (Z_of_var w).
 Proof.
   intros.
-  apply (Zle_trans _ _ _ H).
+  unfold var_max, Zmax, Z_of_var.
+  simpl.
+  destruct ((v ?= w) Eq); reflexivity.
+Qed.
+
+Lemma Zle_Ple : forall p q, Zle (Z_of_var p) (Z_of_var q) -> p <= q.
+Proof.
+  intros. apply H.
+Qed.
+
+Lemma Ple_Zle : forall p q, p <= q -> Zle (Z_of_var p) (Z_of_var q).
+Proof.
+  intros. apply H.
+Qed.
+
+Definition var_list_max := fold_right var_max 1.
+
+Lemma var_max_l : forall x y, x <= var_max x y.
+Proof.
+  intros.
+  apply Zle_Ple.
+  rewrite var_max_hom.
   apply Zle_max_l.
 Qed.
 
-Lemma finite_nat_list_max : forall (l : list Z),
-  { n : Z | forall x, In x l -> x <= n }.
+Lemma finite_var_list_max : forall l x,
+  In x l -> x <= var_list_max l.
 Proof.
-  induction l as [ | l ls IHl ].
-  exists 0; intros x H; inversion H.
-  inversion IHl as [x H].
-  exists (Zmax x l); intros y J; simpl in J; inversion J.
-    subst; apply Zle_max_r.
-    assert (y <= x); auto using max_lt_l.
+  induction l as [ | l ls IHl ]; intros x H.
+    inversion H.
+  simpl.
+  simpl in H; destruct H.
+    subst.
+    apply var_max_l.
+  apply Zle_Ple.
+  rewrite var_max_hom.
+  eapply Zle_trans.
+    apply Ple_Zle. apply IHl. auto.
+  apply Zle_max_r.
 Qed.
 
-Lemma finite_nat_list_max' : forall (l : list Z),
-  { n : Z | ~ In n l }.
-Proof.
-  intros l.
-  case (finite_nat_list_max l); intros x H.
-  exists (x+1).
-  intros J.
-  assert (K := H _ J); omega.
-Qed.
+Definition vars_rep L := var_list_max (S.elements L).
 
-Definition var_generate (L : vars) : var :=
-  proj1_sig (finite_nat_list_max' (S.elements L)).
+Definition var_shift v p := v + p.
+
+Definition var_generate L := var_shift (vars_rep L) 1.
+Lemma InA_In : forall v L, SetoidList.InA E.eq v L -> In v L.
+  induction 1; auto.
+Qed.
 
 Lemma var_generate_spec : forall E, (var_generate E) \notin E.
 Proof.
-  unfold var_generate. intros E.
-  destruct (finite_nat_list_max' (S.elements E)) as [n pf].
-  simpl. intros a.
-  assert (In n (S.elements E)). rewrite <- InA_iff_In.
-  auto using S.elements_1.
-  intuition.
+  unfold var_generate. intros E n.
+  puts (InA_In (S.elements_1 n)).
+  puts (finite_var_list_max _ _ H).
+  unfold var_shift, vars_rep in *.
+  remember (var_list_max (S.elements E)) as x.
+  assert ((Z_of_var x+1 <= Z_of_var x)%Z).
+    apply H0.
+  omega.
 Qed.
 
 Lemma var_fresh : forall (L : vars), { x : var | x \notin L }.
 Proof.
   intros L. exists (var_generate L). apply var_generate_spec.
+Defined.
+
+Lemma elements_singleton : forall v, S.elements {{v}} = v :: nil.
+Proof.
+  intros.
+  generalize (S.elements_1 (S.singleton_2 (refl_equal v))).
+  generalize (S.elements_3w {{v}}).
+  case_eq (S.elements {{v}}); intros.
+    inversion H1.
+  assert (v = e).
+    apply S.singleton_1.
+    apply S.elements_2.
+    rewrite H.
+    constructor. reflexivity.
+  subst e.
+  destruct l. reflexivity.
+  assert (v = e).
+    apply S.singleton_1.
+    apply S.elements_2.
+    rewrite H.
+    apply InA_cons_tl.
+    constructor. reflexivity.
+  subst e.
+  inversion H0.
+  elim H4. constructor. reflexivity.
+Qed.
+
+Lemma var_singleton : forall v, vars_rep {{v}} = v.
+Proof.
+  intros.
+  unfold vars_rep.
+  rewrite elements_singleton.
+  simpl.
+  unfold var_max.
+  destruct v; simpl; auto.
+Qed.
+
+Lemma elements_incl_1 : forall L1 L2,
+  incl (S.elements (L1 \u L2)) (S.elements L1 ++ S.elements L2).
+Proof.
+  introv a H.
+  puts (S.elements_2
+          (@In_InA _ Positive_as_OT.eq Positive_as_OT.eq_refl _ _ H)).
+  destruct (S.union_1 H0); puts (S.elements_1 H1); apply in_or_app.
+    left; apply* InA_In.
+  right; apply* InA_In.
+Qed.
+
+Lemma elements_incl_2 : forall L1 L2,
+  incl (S.elements L1 ++ S.elements L2) (S.elements (L1 \u L2)).
+Proof.
+  introv a H.
+  apply InA_In.
+  apply S.elements_1.
+  destruct (in_app_or _ _ _ H);
+  puts (S.elements_2
+          (@In_InA _ Positive_as_OT.eq Positive_as_OT.eq_refl _ _ H0)).
+    apply* S.union_2.
+  apply* S.union_3.
+Qed.
+
+Require Import Zmax.
+
+Lemma var_list_max_le : forall l1 l2,
+  incl l1 l2 -> var_list_max l1 <= var_list_max l2.
+Proof.
+  intros; induction l1.
+    unfold Ple; destruct (var_list_max l2); intro; discriminate.
+  simpl.
+  apply Zle_Ple. rewrite var_max_hom.
+  apply Zmax_lub.
+    apply Ple_Zle. apply finite_var_list_max. apply* H.
+  apply IHl1.
+  intros b Hb; apply* H.
+Qed.
+
+Lemma var_max_plus_r : forall p q r,
+  var_max p q + r = var_max (p + r) (q + r).
+Proof.
+  intros.
+  unfold var_max.
+  case_eq ((p ?= q) Eq); intros.
+      rewrite (Pcompare_Eq_eq _ _ H).
+      rewrite Pcompare_refl.
+      reflexivity.
+    puts (nat_of_P_lt_Lt_compare_morphism _ _ H).
+    puts (plus_lt_compat_r _ _ (nat_of_P r) H0).
+    repeat rewrite <- nat_of_P_plus_morphism in H1.
+    rewrite (nat_of_P_lt_Lt_compare_complement_morphism _ _ H1).
+    reflexivity.
+  puts (nat_of_P_gt_Gt_compare_morphism _ _ H).
+  puts (plus_lt_compat_r _ _ (nat_of_P r) H0).
+  repeat rewrite <- nat_of_P_plus_morphism in H1.
+  rewrite (nat_of_P_gt_Gt_compare_complement_morphism _ _ H1).
+  reflexivity.
+Qed.
+
+Lemma var_union : forall L1 L2,
+  vars_rep (L1 \u L2) = var_max (vars_rep L1) (vars_rep L2).
+Proof.
+  intros.
+  unfold vars_rep.
+  pose (vlm := fun x => var_list_max (S.elements x)).
+  assert (vlm (L1 \u L2) <= var_max (vlm L1) (vlm L2)).
+    puts (elements_incl_1 L1 L2).
+    unfold vlm.
+    induction (S.elements (L1 \u L2)).
+      apply Zle_Ple.
+      rewrite var_max_hom.
+      destruct (S.elements L1); simpl.
+        apply Zle_max_l.
+      rewrite (var_max_hom e).
+      unfold Z_of_var.
+      apply (Zle_trans 1 (Zpos e)).
+        apply Ple_Zle.
+        unfold Ple.
+        destruct e; simpl; intro; discriminate.
+      eapply Zle_trans. apply Zle_max_l.
+      apply Zle_max_l.
+    simpl.
+    apply Zle_Ple.
+    rewrite var_max_hom.
+    apply Zmax_lub.
+      forward~ (H a) as Ha.
+      rewrite var_max_hom.
+      destruct (in_app_or _ _ _ Ha);
+        puts (Ple_Zle (finite_var_list_max _ _ H0)).
+        eapply Zle_trans. apply H1.
+        apply Zle_max_l.
+      eapply Zle_trans. apply H1.
+      apply Zle_max_r.
+    apply IHl.
+    intros b Hb; apply* H.
+  assert (var_max (vlm L1) (vlm L2) <= vlm (L1 \u L2)).
+    puts (elements_incl_2 L1 L2).
+    unfold vlm.
+    apply Zle_Ple.
+    rewrite var_max_hom.
+    apply Zmax_lub; apply Ple_Zle; apply var_list_max_le;
+      intros a Ha; apply H0; apply* in_or_app.
+  puts (Zle_antisym _ _ (Ple_Zle H) H0).
+  inversion H1.
+  apply H3.
+Qed.
+
+Lemma var_is_fresh : forall L,
+  proj1_sig (var_fresh L) = var_generate L.
+Proof.
+  reflexivity.
+Qed.
+
+Lemma Z_of_var_inj' : forall m n, Z_of_var m = Z_of_var n -> m = n.
+Proof.
+  intros.
+  puts (f_equal var_of_Z H).
+  repeat rewrite Z_of_var_inj in H0.
+  assumption.
+Qed.
+
+Lemma var_add : forall L, vars_rep (L \u {{var_generate L}}) = var_generate L.
+Proof.
+  intros.
+  unfold var_generate.
+  rewrite var_union.
+  rewrite var_singleton.
+  apply Z_of_var_inj'.
+  apply Zle_antisym.
+    rewrite var_max_hom.
+    apply Zmax_lub.
+      unfold var_shift.
+      unfold Z_of_var.
+      rewrite Zpos_plus_distr. omega.
+    apply Zle_refl.
+  rewrite var_max_hom.
+  apply Zle_max_r.
 Qed.
 
 End Variables.
@@ -162,15 +391,32 @@ Qed.
 
 (* It is possible to build a list of n fresh variables. *)
 
+Fixpoint var_nexts v (n:nat) {struct n} : list var :=
+  match n with
+  | 0 => nil
+  | S m => 
+    let v' := var_shift v 1 in
+    v' :: var_nexts v' m
+  end.
+
+Lemma var_nexts_fresh : forall L n,
+  fresh L n (var_nexts (vars_rep L) n).
+Proof.
+  intros.
+  revert L; induction n; intros.
+    simpl*.
+  constructor. apply var_generate_spec.
+  fold (var_generate L).
+  rewrite <- var_add at 2.
+  apply IHn.
+Qed.
+
 Lemma var_freshes : forall L n, 
   { xs : list var | fresh L n xs }.
 Proof.
-  intros. gen L. induction n; intros L.
-  exists* (nil : list var).
-  destruct (var_fresh L) as [x Fr].
-   destruct (IHn (L \u {{x}})) as [xs Frs].
-   exists* (x::xs).
-Qed.
+  intros. exists (var_nexts (vars_rep L) n).
+  apply var_nexts_fresh.
+Defined.
 
 
 (* ********************************************************************** *)
